PAC_Checker2/EPAC_Efficient_Checker.thy
@@ -11,10 +11,46 @@ definition add_poly_l' where
 
 datatype ordered = LESS | EQUAL | GREATER | UNKNOWN
 
+definition perfect_shared_var_order :: \<open>(nat, string)vars \<Rightarrow> string \<Rightarrow> string \<Rightarrow> ordered nres\<close> where
+  \<open>perfect_shared_var_order \<D> x y = do {
+    ASSERT(x \<in># \<D> \<and> y \<in># \<D>);
+    eq \<leftarrow> perfectly_shared_strings_equal \<D> x y;
+    if eq then RETURN EQUAL
+    else do {
+      x \<leftarrow> get_var_name \<D> x;
+      y \<leftarrow> get_var_name \<D> y;
+      if (x, y) \<in> var_order_rel then RETURN (LESS)
+      else RETURN (GREATER)
+    }
+  }\<close>
+
+lemma var_roder_rel_total:
+  \<open>y \<noteq> ya \<Longrightarrow> (y, ya) \<notin> var_order_rel \<Longrightarrow> (ya, y) \<in> var_order_rel\<close>
+  unfolding var_order_rel_def
+  using less_than_char_linear lexord_linear by blast
+
+lemma perfect_shared_var_order_spec:
+  assumes \<open>xs \<in># \<V>\<close>  \<open>ys \<in># \<V>\<close>
+  shows
+    \<open>perfect_shared_var_order \<V> xs ys \<le> \<Down> Id (SPEC(\<lambda>b. ((b=LESS \<longrightarrow> (xs, ys) \<in> var_order_rel) \<and>
+    (b=GREATER \<longrightarrow> (ys, xs) \<in> var_order_rel \<and> \<not>(xs, ys) \<in> var_order_rel) \<and>
+    (b=EQUAL \<longrightarrow> xs = ys)) \<and> b \<noteq> UNKNOWN))\<close>
+  using assms unfolding perfect_shared_var_order_def perfectly_shared_strings_equal_def nres_monad3 get_var_name_def
+  by refine_vcg
+   (auto dest: var_roder_rel_total)
+
+
+definition perfect_shared_term_order_rel_pre
+  :: \<open>(nat, string) vars \<Rightarrow> string list \<Rightarrow> string list \<Rightarrow> bool\<close>
+where
+  \<open>perfect_shared_term_order_rel_pre \<V> xs ys \<longleftrightarrow>
+    set xs \<subseteq> set_mset \<V> \<and> set ys \<subseteq> set_mset \<V>\<close>
+
 definition perfect_shared_term_order_rel
   :: \<open>(nat, string) vars \<Rightarrow> string list \<Rightarrow> string list \<Rightarrow> ordered nres\<close>
 where
   \<open>perfect_shared_term_order_rel \<V> xs ys  = do {
+    ASSERT (perfect_shared_term_order_rel_pre \<V> xs ys);
     (b, _, _) \<leftarrow> WHILE\<^sub>T (\<lambda>(b, xs, ys). b = UNKNOWN)
     (\<lambda>(b, xs, ys). do {
        if xs = [] \<and> ys = [] then RETURN (EQUAL, xs, ys)
@@ -22,22 +58,14 @@ where
        else if ys = [] then RETURN (GREATER, xs, ys)
        else do {
          ASSERT(xs \<noteq> [] \<and> ys \<noteq> []); 
-         eq \<leftarrow> perfectly_shared_strings_equal \<V> (hd xs) (hd ys);
-         if eq then RETURN (b, tl xs, tl ys)
-         else do {
-           x \<leftarrow> get_var_name \<V> (hd xs);
-           y \<leftarrow> get_var_name \<V> (hd ys);
-           if (x, y) \<in> var_order_rel then RETURN (LESS, xs, ys)
-           else RETURN (GREATER, xs, ys)}
-       }
+         eq \<leftarrow> perfect_shared_var_order \<V> (hd xs) (hd ys);
+         if eq = EQUAL then RETURN (b, tl xs, tl ys)
+         else RETURN (eq, xs, ys)
+      }
     }) (UNKNOWN, xs, ys);
     RETURN b
   }\<close>
 
-lemma var_roder_rel_total:
-  \<open>y \<noteq> ya \<Longrightarrow> (y, ya) \<notin> var_order_rel \<Longrightarrow> (ya, y) \<in> var_order_rel\<close>
-  unfolding var_order_rel_def
-  using less_than_char_linear lexord_linear by blast
 
 lemma perfect_shared_term_order_rel_spec:
   assumes \<open>set xs \<subseteq> set_mset \<V>\<close>  \<open>set ys \<subseteq> set_mset \<V>\<close>
@@ -53,7 +81,9 @@ proof -
     unfolding perfect_shared_term_order_rel_def get_var_name_def perfectly_shared_strings_equal_def
       perfectly_shared_strings_equal_def
     apply (refine_vcg WHILET_rule[where I= \<open>I\<close> and
-      R = \<open>measure (\<lambda>(b, xs, ys). length xs + (if b = UNKNOWN then 1 else 0))\<close>])
+      R = \<open>measure (\<lambda>(b, xs, ys). length xs + (if b = UNKNOWN then 1 else 0))\<close>]
+      perfect_shared_var_order_spec[THEN order_trans])
+    subgoal by (auto simp: perfect_shared_term_order_rel_pre_def)
     subgoal by auto
     subgoal by auto
     subgoal by auto
@@ -64,18 +94,11 @@ proof -
     subgoal by auto
     subgoal by (auto simp: neq_Nil_conv lexord_append_leftI)
     subgoal by (auto simp: neq_Nil_conv)
+    subgoal
+      by ((subst conc_Id id_apply)+, rule SPEC_rule, rename_tac x, case_tac x)
+       (auto simp: neq_Nil_conv intro: var_roder_rel_total
+        intro!: lexord_append_leftI lexord_append_rightI)
     subgoal by (auto simp: neq_Nil_conv lexord_append_leftI)
-    subgoal by (auto simp: neq_Nil_conv)
-    subgoal by (auto simp: neq_Nil_conv)
-    subgoal by (auto simp: neq_Nil_conv)
-    subgoal by (auto simp: neq_Nil_conv intro: var_roder_rel_total
-      intro!: lexord_append_leftI lexord_append_rightI)
-    subgoal by (auto simp: neq_Nil_conv intro: var_roder_rel_total
-      intro!: lexord_append_leftI lexord_append_rightI)
-    subgoal by (auto simp: neq_Nil_conv intro: var_roder_rel_total
-      intro!: lexord_append_leftI lexord_append_rightI)
-    subgoal by (auto simp: neq_Nil_conv)
-    subgoal by (auto simp: neq_Nil_conv)
     subgoal by (auto simp: neq_Nil_conv)
     subgoal by (auto simp: neq_Nil_conv)
     subgoal by (auto simp: neq_Nil_conv)
@@ -92,7 +115,7 @@ lemma term_order_rel_irreflexive:
   using lexord_trans[of x1f x1d var_order_rel x1f] lexord_irreflexive[of var_order_rel x1f]
   by simp
 
-definition add_poly_l_prep :: \<open>(nat,string)vars \<Rightarrow> llist_polynomial \<times> llist_polynomial \<Rightarrow>  llist_polynomial nres\<close> where
+definition add_poly_l_prep :: \<open>(nat,string)vars \<Rightarrow> llist_polynomial \<times> llist_polynomial \<Rightarrow> llist_polynomial nres\<close> where
   \<open>add_poly_l_prep \<D> = REC\<^sub>T
   (\<lambda>add_poly_l (p, q).
   case (p,q) of
@@ -197,8 +220,6 @@ definition linear_combi_l_prep where
         })
         ([], xs, CSUCCESS)
         }\<close>
-        find_theorems import_poly_no_new
-          term import_poly_no_new
 
 
 lemma import_poly_no_new_spec:
@@ -282,6 +303,257 @@ proof -
     done 
 qed
 
+thm mult_poly_full_def
+thm mult_poly_raw_def
+thm mult_monomials_def
+thm mult_monoms.simps
+term REC\<^sub>T
+
+definition mult_monoms_prep :: \<open>(nat,string)vars \<Rightarrow> term_poly_list \<Rightarrow> term_poly_list \<Rightarrow> term_poly_list nres\<close> where
+  \<open>mult_monoms_prep \<D> xs ys = REC\<^sub>T (\<lambda>f (xs, ys).
+ do {
+    if xs = [] then RETURN ys
+    else if ys = [] then RETURN xs
+    else do {
+      ASSERT(xs \<noteq> [] \<and> ys \<noteq> []);
+      comp \<leftarrow> perfect_shared_var_order \<D> (hd xs) (hd ys);
+      if comp = EQUAL then do {
+        pq \<leftarrow> f (tl xs, tl ys);
+        RETURN (hd xs # pq)
+      }
+      else if comp = LESS then do {
+        pq \<leftarrow> f (tl xs, ys);
+        RETURN (hd xs # pq)
+      }
+      else do {
+        pq \<leftarrow> f (xs, tl ys);
+        RETURN (hd ys # pq)
+      }
+   }
+ }) (xs, ys)\<close>
+
+
+lemma mult_monoms_prep_mult_monoms:
+  assumes \<open>set xs \<subseteq> set_mset \<V>\<close> \<open>set ys \<subseteq> set_mset \<V>\<close>
+  shows \<open>mult_monoms_prep \<V> xs ys \<le> \<Down>Id (SPEC ((=) (mult_monoms xs ys)))\<close>
+proof -
+  have H: \<open>f \<le> RES p \<Longrightarrow> (\<And>x. x \<in> p \<Longrightarrow> (g x) \<in> Q) \<Longrightarrow> do {x \<leftarrow> f; RETURN (g x)} \<le> RES Q\<close> for f p g Q
+    by (meson bind_le_nofailI le_RES_nofailI nres_order_simps(21) order.trans)
+  have [dest]: \<open> (x, y) \<in> var_order_rel \<Longrightarrow>
+    (y, x) \<in> var_order_rel \<Longrightarrow> x = y\<close> for x y
+     by (meson transE trans_var_order_rel var_order_rel_antisym)
+
+  have [dest]: \<open> xa \<noteq> UNKNOWN \<Longrightarrow> xa \<noteq> GREATER \<Longrightarrow> xa \<noteq> LESS \<Longrightarrow> xa = EQUAL \<close> for xa
+    by (cases xa) auto
+  show ?thesis
+   using assms
+    apply (induction xs ys rule:mult_monoms.induct)
+    subgoal
+      unfolding mult_monoms_prep_def
+      by (subst RECT_unfold, refine_mono) auto
+    subgoal
+      unfolding mult_monoms_prep_def
+      by (subst RECT_unfold, refine_mono) auto
+    subgoal
+      apply (subst mult_monoms_prep_def)
+      apply (subst RECT_unfold, refine_mono)
+      apply (subst mult_monoms_prep_def[symmetric])+
+        apply (simp only: prod.simps)
+        apply (refine_vcg perfect_shared_term_order_rel_spec[THEN order_trans]
+          perfect_shared_var_order_spec[THEN order_trans])
+       subgoal by auto
+       subgoal by auto
+       subgoal by auto
+       subgoal by auto
+       subgoal by (auto intro!: H)
+       done
+    done
+qed
+
+definition mult_monoms_prop :: \<open>(nat,string)vars\<Rightarrow> llist_polynomial \<Rightarrow>  _ \<Rightarrow> llist_polynomial \<Rightarrow> llist_polynomial nres\<close> where
+  \<open>mult_monoms_prop = (\<lambda>\<V> qs (p, m) b. nfoldli qs (\<lambda>_. True) (\<lambda>(q, n) b. do {pq \<leftarrow> mult_monoms_prep \<V> p q; RETURN ((pq, m * n) # b)}) b)\<close>
+
+definition mult_poly_raw_prop :: \<open>(nat,string) vars\<Rightarrow> llist_polynomial \<Rightarrow> llist_polynomial \<Rightarrow> llist_polynomial nres\<close> where
+  \<open>mult_poly_raw_prop \<V> p q = nfoldli p (\<lambda>_. True) (mult_monoms_prop \<V> q) []\<close>
+
+lemma mult_monoms_prop_mult_monomials:
+  assumes \<open>vars_llist qs \<subseteq> set_mset \<V>\<close> \<open>set (fst m) \<subseteq> set_mset \<V>\<close>
+  shows \<open>mult_monoms_prop \<V> qs m b \<le> \<Down>{(xs, ys). mset xs = mset ys} (RES{map (mult_monomials m) qs @ b})\<close>
+    using assms
+  unfolding mult_monoms_prop_def
+  apply (cases m)
+  apply (induction qs arbitrary: b)
+  subgoal by (auto intro!: RETURN_RES_refine)
+  subgoal for a qs aa b ba
+    apply (cases a)
+    apply (simp only: prod.simps nfoldli_simps(2) if_True nres_monad3 nres_monad1)
+    apply (refine_vcg mult_monoms_prep_mult_monoms[THEN order_trans])
+    subgoal by auto
+    subgoal by auto
+    subgoal premises p
+      supply [intro!] = p(1)[THEN order_trans]
+      using p(2-)
+      by (auto simp: conc_fun_RES mult_monomials_def)
+    done
+  done
+
+
+lemma mult_poly_raw_prop_mult_poly_raw:
+  assumes \<open>vars_llist qs \<subseteq> set_mset \<V>\<close> \<open>vars_llist ps \<subseteq> set_mset \<V>\<close>
+  shows \<open>mult_poly_raw_prop \<V> ps qs \<le>
+       (SPEC (\<lambda>c. (c, PAC_Polynomials_Operations.mult_poly_raw ps qs) \<in> {(xs, ys). mset xs = mset ys}))\<close>
+proof -
+  have [simp]: \<open>foldl (\<lambda>b x. map (mult_monomials x) qs @ b) b ps = foldl (\<lambda>b x. map (mult_monomials x) qs @ b) [] ps @ b\<close>
+    if \<open>NO_MATCH [] b\<close> for qs ps b
+    apply (induction ps arbitrary: b)
+      apply simp
+    by (metis (no_types, lifting) append_assoc foldl_Cons self_append_conv)
+
+
+  have H: \<open>nfoldli ps (\<lambda>_. True) (mult_monoms_prop \<V> qs) b0
+    \<le> \<Down> {(xs, ys). mset xs = mset ys} (RES {foldl (\<lambda>b x. map (mult_monomials x) qs @ b) b0 ps})\<close> for b0
+    using assms
+    apply (induction ps arbitrary: b0)
+    subgoal by (auto intro!: RETURN_RES_refine)
+    subgoal premises p
+      supply [intro!] = p(1)[THEN order_trans]
+      using p(2-)
+      apply (simp only: prod.simps nfoldli_simps(2) if_True nres_monad3 nres_monad1)
+      apply (refine_rcg mult_monoms_prop_mult_monomials)
+      apply auto
+      apply (rule specify_left)
+      apply (subst RES_SPEC_eq[symmetric])
+      apply (rule mult_monoms_prop_mult_monomials[unfolded conc_fun_RES])
+      apply (auto simp: conc_fun_RES)
+      done
+    done
+
+  show ?thesis
+    unfolding mult_poly_raw_def mult_poly_raw_prop_def
+    by (rule H[THEN order_trans]) (auto simp: conc_fun_RES)
+qed
+
+definition mult_poly_full_prop :: \<open>_\<close> where
+\<open>mult_poly_full_prop \<V> p q = do {
+  pq \<leftarrow> mult_poly_raw_prop \<V> p q;
+  normalize_poly pq
+}\<close>
+
+lemma mult_poly_full_prop_mult_poly_full:
+  assumes \<open>vars_llist qs \<subseteq> set_mset \<V>\<close> \<open>vars_llist ps \<subseteq> set_mset \<V>\<close>
+  shows \<open>mult_poly_full_prop \<V> ps qs \<le> \<Down>Id (mult_poly_full ps qs)\<close>
+proof -
+  have [refine0]: \<open>sort_poly_spec p \<le> \<Down> Id (sort_poly_spec p')\<close>
+    if \<open>mset p= mset p'\<close> for p p'
+    using that
+    unfolding sort_poly_spec_def
+    by auto
+  show ?thesis
+    using assms
+    unfolding mult_poly_full_prop_def mult_poly_full_def normalize_poly_def
+    by (refine_vcg mult_poly_raw_prop_mult_poly_raw) auto
+qed
+  term linear_combi_l_prep
+thm linear_combi_l_prep_def
+definition linear_combi_l_prep2 where
+\<open>linear_combi_l_prep2 i A \<V> xs = do {
+    WHILE\<^sub>T
+      (\<lambda>(p, xs, err). xs \<noteq> [] \<and> \<not>is_cfailed err)
+      (\<lambda>(p, xs, _). do {
+         ASSERT(xs \<noteq> []);
+         let (q\<^sub>0 :: llist_polynomial, i) = hd xs;
+         if (i \<notin># dom_m A \<or> \<not>(vars_llist q\<^sub>0 \<subseteq> set_mset \<V>))
+         then do {
+           err \<leftarrow> check_linear_combi_l_dom_err q\<^sub>0 i;
+           RETURN (p, xs, error_msg i err)
+         } else do {
+           ASSERT(fmlookup A i \<noteq> None);
+           let r = the (fmlookup A i);
+           (_, q) \<leftarrow> normalize_poly_shared \<V> (q\<^sub>0);
+           ASSERT(vars_llist q \<subseteq> set_mset \<V>);
+           pq \<leftarrow> mult_poly_full_prop \<V> q r;
+           pq \<leftarrow> add_poly_l_prep \<V> (p, pq);
+           RETURN (pq, tl xs, CSUCCESS)
+         }
+      })
+     ([], xs, CSUCCESS)
+    }\<close>
+
+lemma
+  assumes \<V>: \<open>(\<V>,\<V>') \<in> {(x, y). y = set_mset x}\<close> and
+    A: \<open>\<And>xs. xs \<in># dom_m A \<Longrightarrow> vars_llist (A \<propto> xs) \<subseteq> set_mset \<V>\<close>
+  shows \<open>linear_combi_l_prep2 i A \<V> xs \<le> \<Down>Id (linear_combi_l i A \<V>' xs)\<close>
+proof -
+  have H1: \<open>(if p \<or> q then P else Q) = (if p then P else if q then P else Q)\<close> for p q P Q
+    by auto
+  have [intro!]: \<open>check_linear_combi_l_dom_err x1e x2e \<le> \<Down> Id (check_linear_combi_l_dom_err x1e x2e)\<close>
+    for x1e x2e
+    by auto
+  have linear_combi_l_alt_def:
+      \<open>linear_combi_l i A \<V> xs = do {
+      WHILE\<^sub>T
+        (\<lambda>(p, xs, err). xs \<noteq> [] \<and> \<not>is_cfailed err)
+        (\<lambda>(p, xs, _). do {
+          ASSERT(xs \<noteq> []);
+          let (q :: llist_polynomial, i) = hd xs;
+          if (i \<notin># dom_m A \<or> \<not>(vars_llist q \<subseteq> \<V>))
+          then do {
+            err \<leftarrow> check_linear_combi_l_dom_err q i;
+            RETURN (p, xs, error_msg i err)
+            }
+          else do {
+          ASSERT(fmlookup A i \<noteq> None);
+          let r = the (fmlookup A i);
+          q \<leftarrow> full_normalize_poly q;
+          ASSERT (vars_llist q \<subseteq> \<V>);
+          let q = q;
+          pq \<leftarrow> mult_poly_full q r;
+          pq \<leftarrow> add_poly_l' \<V>' (p, pq);
+          RETURN (pq, tl xs, CSUCCESS)
+          }
+       })
+    ([], xs, CSUCCESS)
+    }\<close> for i A \<V> xs
+    unfolding Let_def linear_combi_l_def add_poly_l'_def by auto
+  have H: \<open>P = Q \<Longrightarrow> P \<le>\<Down>Id Q\<close> for P Q
+    by auto
+  have [refine0]: \<open>\<Down> Id (SPEC (\<lambda>(b, xs'). (\<not> b \<longrightarrow> xa = xs') \<and> (\<not> b) = (vars_llist xa \<subseteq> set_mset \<V>)))
+    \<le> SPEC (\<lambda>c. (c, q) \<in> {((b, c), d). \<not>b \<and> c = d \<and> d = q})\<close>
+    if \<open>vars_llist xa \<subseteq> set_mset \<V>\<close> \<open>xa = q\<close>
+    for xa \<V> q
+    using that by auto
+  show ?thesis
+    unfolding linear_combi_l_prep2_def linear_combi_l_alt_def normalize_poly_shared_def nres_monad3
+    apply (refine_rcg import_poly_no_new_spec[THEN order_trans]
+      mult_poly_full_prop_mult_poly_full[THEN order_trans]
+      add_poly_alt_def[THEN order_trans])
+    subgoal by auto
+    subgoal by auto
+    subgoal by auto
+    subgoal using \<V> by auto
+    apply (rule H)
+    subgoal by auto
+    subgoal by auto
+    subgoal by auto
+    apply (rule H)
+    subgoal by auto
+    subgoal using \<V> by auto
+    subgoal by auto
+    subgoal using \<V> by auto
+    subgoal using \<V> A by auto
+    apply (rule H)
+    subgoal by auto
+    subgoal using \<V> A apply auto
+      sorry
+    subgoal using \<V> A apply auto
+      sorry
+    apply (rule H)
+    subgoal by (auto simp: add_poly_l'_def)
+    subgoal by auto
+    done
+qed
+    find_theorems linear_combi_l_prep
+oops
 end
 
 end
